some setoid stuff prototyping for maps

coq/SigmaHCOL/MemVecEq.v
@@ -49,6 +49,104 @@ Definition svector_to_mem_block {fm} {n}:=
 Global Instance mem_block_Equiv:
   Equiv (mem_block) := mem_block_equiv.
 
+Require Import Coq.FSets.FMapFacts.
+Module NMF := WFacts_fun Coq.Structures.OrderedTypeEx.Nat_as_OT NM.
+
+Definition NatMap := NM.t.
+
+Definition CarrierA_beq (a b: CarrierA) : bool
+  := bool_decide (a=b).
+
+Global Instance mem_block_Equiv_Reflexive:
+  Reflexive (mem_block_Equiv).
+Proof.
+  intros x.
+  unfold mem_block_Equiv, mem_block_equiv.
+  rewrite NMF.Equiv_Equivb with (cmp:=CarrierA_beq).
+  -
+    unfold NM.Equivb, CarrierA_beq, NM.Equiv, bool_decide.
+    split.
+    +
+      reflexivity.
+    +
+      intros k e e' H0 H1.
+      unfold Cmp.
+      break_if.
+      * reflexivity.
+      *
+        clear Heqd.
+        apply NMF.MapsTo_fun with (e:=e') in H0.
+        rewrite H0 in n.
+        auto.
+        apply H1.
+  -
+    split.
+    +
+      unfold CarrierA_beq, bool_decide.
+      break_if.
+      auto.
+      intros.
+      congruence.
+    +
+      intros H.
+      unfold CarrierA_beq, bool_decide.
+      break_if.
+      auto.
+      contradiction n.
+Qed.
+
+Global Instance mem_block_Equiv_Symmetric:
+  Symmetric (mem_block_Equiv).
+Proof.
+  intros x y.
+  unfold mem_block_Equiv, mem_block_equiv.
+Admitted.
+
+Global Instance mem_block_Equiv_Transitive:
+  Transitive (mem_block_Equiv).
+Proof.
+  intros x y z.
+  unfold mem_block_Equiv, mem_block_equiv.
+Admitted.
+
+Global Instance mem_block_Equiv_Equivalence:
+  Equivalence (mem_block_Equiv).
+Proof.
+  split.
+  apply mem_block_Equiv_Reflexive.
+  apply mem_block_Equiv_Symmetric.
+  apply mem_block_Equiv_Transitive.
+Qed.
+
+Global Instance avector_to_mem_block_Proper {n}:
+  Proper ((=) ==> (=)) (@avector_to_mem_block n).
+Proof.
+  simpl_relation.
+  induction n.
+  -
+    dep_destruct x.
+    dep_destruct y.
+    split.
+    +
+      crush.
+    +
+      intros;simpl.
+      unfold avector_to_mem_block in *.
+      unfold mem_empty in *.
+      apply NMF.empty_mapsto_iff in H0.
+      destruct H0.
+  -
+    split.
+    +
+      intros.
+      dep_destruct x. clear x. rename h into xh, x0 into xs.
+      dep_destruct y. clear y. rename h into yh, x into ys.
+      apply Vcons_equiv_elim in H.
+      destruct H as [Hh Ht].
+      specialize (IHn xs ys Ht).
+      destruct IHn as [IHn0 IHn1].
+Qed.
+
 Class SHOperator_MemVecEq
       {fm}
       {i o: nat}
@@ -62,3 +160,65 @@ Class SHOperator_MemVecEq
           mem_op fm f (svector_to_mem_block x)
       ;
     }.
+
+
+Section MemVecEq.
+  Variable fm:Monoid RthetaFlags.
+  Variable fml:@MonoidLaws RthetaFlags RthetaFlags_type fm.
+
+  Global Instance liftM_MemVecEq
+         {i o}
+         (hop: avector i -> avector o)
+         `{HOP: HOperator i o hop}
+    : SHOperator_MemVecEq (liftM_HOperator fm hop).
+  Proof.
+    assert (facts: SHOperator_Facts fm (liftM_HOperator fm hop)) by
+        typeclasses eauto.
+    split.
+    intros x.
+    simpl.
+    unfold mem_op_of_hop.
+    unfold liftM_HOperator', compose.
+
+    induction x.
+    -
+      simpl.
+      f_equiv.
+      induction (hop Vnil).
+      +
+        simpl.
+        unfold svector_to_mem_block, compose.
+        reflexivity.
+      +
+        simpl.
+        unfold svector_to_mem_block, compose in *.
+        simpl in *.
+
+    -
+      simpl.
+
+
+
+
+    induction i.
+    -
+      simpl.
+      f_equiv.
+      dep_destruct x. clear x.
+      induction o.
+      +
+        dep_destruct (hop Vnil).
+        dep_destruct (liftM_HOperator' (fm:=fm) hop Vnil).
+        unfold svector_to_mem_block, compose.
+        simpl.
+        reflexivity.
+      +
+        dep_destruct (hop Vnil).
+        admit.
+    -
+      destruct x.
+      admit.
+      admit.
+  Admitted.
+
+End MemVecEq.
